backends/lean/Aeneas/ScalarTac/Lemmas.lean
@@ -63,6 +63,7 @@ theorem Usize.cMax_bound : UScalar.cMax .Usize ≤ Usize.max ∧ Usize.max + 1 =
   have := System.Platform.numBits_eq; cases this <;> simp [*]
 
 grind_pattern Usize.cMax_bound => Usize.max
+grind_pattern [agrind] Usize.cMax_bound => Usize.max
 
 @[scalar_tac Usize.size]
 theorem Usize.size_scalarTac_eq : Usize.size = Usize.max + 1 ∧ Usize.size = 2^System.Platform.numBits := by
@@ -70,18 +71,21 @@ theorem Usize.size_scalarTac_eq : Usize.size = Usize.max + 1 ∧ Usize.size = 2^
   have := System.Platform.numBits_eq; cases this <;> simp [*]
 
 grind_pattern Usize.size_scalarTac_eq => Usize.size
+grind_pattern [agrind] Usize.size_scalarTac_eq => Usize.size
 
 abbrev Usize.maxAbbrevPow := 2^System.Platform.numBits
 @[scalar_tac Usize.maxAbbrevPow]
 theorem Usize.cMax_bound' : UScalar.cMax .Usize ≤ Usize.max ∧ Usize.max + 1 = 2^System.Platform.numBits := Usize.cMax_bound
 
 grind_pattern Usize.cMax_bound' => Usize.maxAbbrevPow
+grind_pattern [agrind] Usize.cMax_bound' => Usize.maxAbbrevPow
 
 abbrev Usize.maxAbbrevPow' := 2^Usize.numBits
 @[scalar_tac Usize.maxAbbrevPow']
 theorem Usize.cMax_bound'' : UScalar.cMax .Usize ≤ Usize.max ∧ Usize.max + 1 = 2^System.Platform.numBits := Usize.cMax_bound
 
 grind_pattern Usize.cMax_bound'' => Usize.maxAbbrevPow'
+grind_pattern [agrind] Usize.cMax_bound'' => Usize.maxAbbrevPow'
 
 @[scalar_tac Isize.min]
 theorem Isize.cMin_bound : Isize.min ≤ IScalar.cMin .Isize ∧ Isize.min = - 2^(System.Platform.numBits - 1) := by
@@ -89,18 +93,21 @@ theorem Isize.cMin_bound : Isize.min ≤ IScalar.cMin .Isize ∧ Isize.min = - 2
   have := System.Platform.numBits_eq; cases this <;> simp [*]
 
 grind_pattern Isize.cMin_bound => Isize.min
+grind_pattern [agrind] Isize.cMin_bound => Isize.min
 
 abbrev Isize.minAbbrevPow :Int := -2^(System.Platform.numBits-1)
 @[scalar_tac Isize.minAbbrevPow]
 theorem Isize.cMin_bound' : Isize.min ≤ IScalar.cMin .Isize ∧ Isize.min = - 2^(System.Platform.numBits - 1) := Isize.cMin_bound
 
 grind_pattern Isize.cMin_bound' => Isize.minAbbrevPow
+grind_pattern [agrind] Isize.cMin_bound' => Isize.minAbbrevPow
 
 abbrev Isize.minAbbrevPow' :Int := -2^(Isize.numBits-1)
 @[scalar_tac Isize.minAbbrevPow']
 theorem Isize.cMin_bound'' : Isize.min ≤ IScalar.cMin .Isize ∧ Isize.min = - 2^(System.Platform.numBits - 1) := Isize.cMin_bound
 
 grind_pattern Isize.cMin_bound'' => Isize.minAbbrevPow'
+grind_pattern [agrind] Isize.cMin_bound'' => Isize.minAbbrevPow'
 
 @[scalar_tac Isize.max]
 theorem Isize.cMax_bound : IScalar.cMax .Isize ≤ Isize.max ∧ Isize.max + 1 = 2^(System.Platform.numBits - 1) := by
@@ -108,24 +115,28 @@ theorem Isize.cMax_bound : IScalar.cMax .Isize ≤ Isize.max ∧ Isize.max + 1 =
   have := System.Platform.numBits_eq; cases this <;> simp [*]
 
 grind_pattern Isize.cMax_bound => Isize.max
+grind_pattern [agrind] Isize.cMax_bound => Isize.max
 
 @[scalar_tac Usize.size]
 theorem Isize.size_scalarTac_eq : Isize.size = 2^System.Platform.numBits := by
   simp [Isize.numBits, Isize.size]
 
 grind_pattern Isize.size_scalarTac_eq => Isize.size
+grind_pattern [agrind] Isize.size_scalarTac_eq => Isize.size
 
 abbrev Isize.maxAbbrevPow : Int := 2^(System.Platform.numBits-1)
 @[scalar_tac Isize.maxAbbrevPow]
 theorem Isize.cMax_bound' : IScalar.cMax .Isize ≤ Isize.max ∧ Isize.max + 1 = 2^(System.Platform.numBits - 1) := Isize.cMax_bound
 
 grind_pattern Isize.cMax_bound' => Isize.maxAbbrevPow
+grind_pattern [agrind] Isize.cMax_bound' => Isize.maxAbbrevPow
 
 abbrev Isize.maxAbbrevPow' : Int := 2^(Isize.numBits-1)
 @[scalar_tac Isize.maxAbbrevPow']
 theorem Isize.cMax_bound'' : IScalar.cMax .Isize ≤ Isize.max ∧ Isize.max + 1 = 2^(System.Platform.numBits - 1) := Isize.cMax_bound
 
 grind_pattern Isize.cMax_bound'' => Isize.maxAbbrevPow'
+grind_pattern [agrind] Isize.cMax_bound'' => Isize.maxAbbrevPow'
 
 @[scalar_tac_simps] theorem U8.numBits_eq    : U8.numBits = 8 := by simp_scalar_consts
 @[scalar_tac_simps] theorem U16.numBits_eq   : U16.numBits = 16 := by simp_scalar_consts
@@ -230,6 +241,7 @@ theorem UScalar.bounds {ty : UScalarTy} (x : UScalar ty) :
   omega
 
 grind_pattern UScalar.bounds => UScalar.val x
+grind_pattern [agrind] UScalar.bounds => UScalar.val x
 
 @[scalar_tac x.val]
 theorem IScalar.bounds {ty : IScalarTy} (x : IScalar ty) :
@@ -239,6 +251,7 @@ theorem IScalar.bounds {ty : IScalarTy} (x : IScalar ty) :
   omega
 
 grind_pattern IScalar.bounds => IScalar.val x
+grind_pattern [agrind] IScalar.bounds => IScalar.val x
 
 attribute [scalar_tac a.toNat] Int.toNat_eq_max
 
@@ -264,13 +277,13 @@ attribute [scalar_tac_simps, simp_lists_hyps_simps, simp_scalar_hyps_simps] Int.
 -/
 
 -- TODO: commit to Mathlib
-attribute [scalar_tac_simps, grind =] Nat.shiftLeft_eq Int.shiftLeft_eq
+attribute [scalar_tac_simps, grind =, agrind =] Nat.shiftLeft_eq Int.shiftLeft_eq
 
 @[scalar_tac_simps] theorem Nat.max_eq_Max_max (x y : Nat) : Nat.max x y = x ⊔ y := by simp
 @[scalar_tac_simps] theorem Nat.min_eq_Min_min (x y : Nat) : Nat.min x y = x ⊓ y := by simp
 
 -- TODO: commit to Mathlib
-attribute [grind! .] inf_le_left inf_lt_left inf_le_right inf_lt_right
+attribute [grind! ., agrind! .] inf_le_left inf_lt_left inf_le_right inf_lt_right
 
 example (x y : Nat) : x ≤ x ⊔ y := by scalar_tac
 example (x y : Nat) : x ≤ Nat.max x y := by scalar_tac
@@ -377,24 +390,64 @@ theorem lt_mul_lt_le (x y a b : ℕ) (h0 : x < a) (h1 : y < b) :
   x * y ≤ (a - 1) * (b - 1) := by apply Nat.le_mul_le; omega
 
 grind_pattern lt_mul_lt_le => x * y, x < a, y < b
+  where
+    guard x < a
+    guard y < b
+    gen < 2
+
+grind_pattern [agrind] lt_mul_lt_le => x * y, x < a, y < b
+  where
+    guard x < a
+    guard y < b
+    gen < 2
 
 @[scalar_tac x * y]
 theorem le_mul_lt_le (x y a b : ℕ) (h0 : x ≤ a) (h1 : y < b) :
   x * y ≤ a * (b - 1) := by apply Nat.le_mul_le; omega
 
 grind_pattern le_mul_lt_le => x * y, x ≤ a, y < b
+  where
+    guard x ≤ a
+    guard y < b
+    gen < 2
+
+grind_pattern [agrind] le_mul_lt_le => x * y, x ≤ a, y < b
+  where
+    guard x ≤ a
+    guard y < b
+    gen < 2
 
 @[scalar_tac x * y]
 theorem lt_mul_le_le (x y a b : ℕ) (h0 : x < a) (h1 : y ≤ b) :
   x * y ≤ (a - 1) * b := by apply Nat.le_mul_le; omega
 
 grind_pattern lt_mul_le_le => x * y, x < a, y ≤ b
+  where
+    guard x < a
+    guard y ≤ b
+    gen < 2
+
+grind_pattern [agrind] lt_mul_le_le => x * y, x < a, y ≤ b
+  where
+    guard x < a
+    guard y ≤ b
+    gen < 2
 
 @[scalar_tac x * y]
 theorem le_mul_le_le (x y a b : ℕ) (h0 : x ≤ a) (h1 : y ≤ b) :
   x * y ≤ a * b := by apply Nat.le_mul_le; omega
 
 grind_pattern le_mul_le_le => x * y, x ≤ a, y ≤ b
+  where
+    guard x ≤ a
+    guard y ≤ b
+    gen < 2
+
+grind_pattern [agrind] le_mul_le_le => x * y, x ≤ a, y ≤ b
+  where
+    guard x ≤ a
+    guard y ≤ b
+    gen < 2
 
 /-!
 Not activating those lemmas for now, because there are a lot of them
@@ -471,6 +524,7 @@ example (i j n1 n2 : ℕ)
 theorem mod_lt (x y : ℕ) (h : 0 < y) : x % y < y := by exact Nat.mod_lt x h
 
 grind_pattern mod_lt => x % y
+grind_pattern [agrind] mod_lt => x % y
 
 /-!
 # Size
@@ -478,7 +532,7 @@ grind_pattern mod_lt => x % y
 
 /- Remark: we're omitting a similar theorem for `IScalar` because the theorem is a bit cumbersome
    to use (it has to be expressed in terms of `x.bv.toNat`). -/
-@[scalar_tac_simps, grind =]
+@[scalar_tac_simps, grind =, agrind =]
 theorem UScalar.sizeOf {ty} (x : UScalar ty) : sizeOf x = x.val + 3 := by
   cases x; simp only [UScalar.mk.sizeOf_spec, BitVec.sizeOf, Fin.sizeOf, BitVec.val_toFin]
   unfold UScalar.val
