backends/lean/Aeneas/Std/Array/Array.lean
@@ -27,14 +27,14 @@ instance [BEq α] [LawfulBEq α] : LawfulBEq (Array α n) := SubtypeLawfulBEq _
 def Array.empty (α : Type u) : Array α (Usize.ofNat 0) := ⟨ [], by simp ⟩
 
 /- Registering some theorems for `scalar_tac` -/
-@[scalar_tac_simps, grind =]
+@[scalar_tac_simps, grind =, agrind =]
 theorem Array.length_eq {α : Type u} {n : Usize} (a : Array α n) : a.val.length = n.val := by
   cases a; simp[*]
 
-@[simp, scalar_tac_simps, simp_scalar_simps, simp_lists_simps, grind]
+@[simp, scalar_tac_simps, simp_scalar_simps, simp_lists_simps, grind, agrind]
 abbrev Array.length {α : Type u} {n : Usize} (v : Array α n) : Nat := v.val.length
 
-@[simp, scalar_tac_simps, simp_scalar_simps, simp_lists_simps, grind]
+@[simp, scalar_tac_simps, simp_scalar_simps, simp_lists_simps, grind, agrind]
 abbrev Array.v {α : Type u} {n : Usize} (v : Array α n) : List α := v.val
 
 example {α: Type u} {n : Usize} (v : Array α n) : v.length ≤ Usize.max := by
@@ -61,10 +61,10 @@ example : Result (Array Int (Usize.ofNat 2)) := do
 @[reducible] instance {α : Type u} {n : Usize} : GetElem? (Array α n) Nat α (fun a i => i < a.val.length) where
   getElem? a i := getElem? a.val i
 
-@[simp, scalar_tac_simps, simp_lists_hyps_simps, grind =]
+@[simp, scalar_tac_simps, simp_lists_hyps_simps, grind =, agrind =]
 theorem Array.getElem?_Nat_eq {α : Type u} {n : Usize} (v : Array α n) (i : Nat) : v[i]? = v.val[i]? := by rfl
 
-@[simp, scalar_tac_simps, simp_lists_hyps_simps, grind = _]
+@[simp, scalar_tac_simps, simp_lists_hyps_simps, grind = _, agrind = _]
 theorem Array.getElem!_Nat_eq {α : Type u} [Inhabited α] {n : Usize} (v : Array α n) (i : Nat) : v[i]! = v.val[i]! := by
   simp only [instGetElem?ArrayNatLtLengthValListEqVal, List.getElem!_eq_getElem?_getD]; split <;> simp_all
   rfl
@@ -80,8 +80,8 @@ theorem Array.getElem!_Nat_eq {α : Type u} [Inhabited α] {n : Usize} (v : Arra
   simp [instGetElem?ArrayUsizeLtNatValLengthValListEq]; split <;> simp_all
   rfl
 
-@[simp, scalar_tac_simps, simp_lists_hyps_simps, grind] abbrev Array.get? {α : Type u} {n : Usize} (v : Array α n) (i : Nat) : Option α := getElem? v i
-@[simp, scalar_tac_simps, simp_lists_hyps_simps, grind] abbrev Array.get! {α : Type u} {n : Usize} [Inhabited α] (v : Array α n) (i : Nat) : α := getElem! v i
+@[simp, scalar_tac_simps, simp_lists_hyps_simps, grind, agrind] abbrev Array.get? {α : Type u} {n : Usize} (v : Array α n) (i : Nat) : Option α := getElem? v i
+@[simp, scalar_tac_simps, simp_lists_hyps_simps, grind, agrind] abbrev Array.get! {α : Type u} {n : Usize} [Inhabited α] (v : Array α n) (i : Nat) : α := getElem! v i
 
 @[simp]
 abbrev Array.slice {α : Type u} {n : Usize} [Inhabited α] (v : Array α n) (i j : Nat) : List α :=
@@ -116,17 +116,17 @@ def Array.set {α : Type u} {n : Usize} (v: Array α n) (i: Usize) (x: α) : Arr
 def Array.set_opt {α : Type u} {n : Usize} (v: Array α n) (i: Usize) (x: Option α) : Array α n :=
   ⟨ v.val.set_opt i.val x, by have := v.property; simp [*] ⟩
 
-@[simp, scalar_tac_simps, simp_lists_hyps_simps, grind =]
+@[simp, scalar_tac_simps, simp_lists_hyps_simps, grind =, agrind =]
 theorem Array.set_val_eq {α : Type u} {n : Usize} (v: Array α n) (i: Usize) (x: α) :
   (v.set i x).val = v.val.set i.val x := by
   simp [set]
 
-@[simp, scalar_tac_simps, simp_lists_hyps_simps, grind =]
+@[simp, scalar_tac_simps, simp_lists_hyps_simps, grind =, agrind =]
 theorem Array.set_opt_val_eq {α : Type u} {n : Usize} (v: Array α n) (i: Usize) (x: Option α) :
   (v.set_opt i x).val = v.val.set_opt i.val x := by
   simp [set_opt]
 
-@[scalar_tac_simps, grind =]
+@[scalar_tac_simps, grind =, agrind =]
 theorem Array.set_length {α : Type u} {n : Usize} (v: Array α n) (i: Usize) (x: α) :
   (v.set i x).length = v.length := by simp
 
